verified InsertList together with insert/size

src/Std/Data/DHashMap/Internal/Defs.lean
@@ -353,12 +353,12 @@ where
   return r
 
 /-- Internal implementation detail of the hash map -/
-def insertManyList [BEq α] [Hashable α]
+def insertList [BEq α] [Hashable α]
     (m : Raw₀ α β) (l : List ((a : α) × β a)) : Raw₀ α β := Id.run do
-let mut r := m
-for ⟨a,b⟩ in l do
-  r:= r.insert a b
-return r
+  let mut r := m
+  for ⟨a,b⟩ in l do
+    r:= r.insert a b
+  return r
 
 section
 
