src/Std/Data/DHashMap/Internal/WF.lean
@@ -706,39 +706,39 @@ theorem wfImp_filter [BEq α] [Hashable α] [EquivBEq α] [LawfulHashable α] {m
   rw [filter_eq_filterₘ]
   exact wfImp_filterₘ h
 
-/-! # `insertManyListₘ` -/
-theorem wfImp_insertManyListₘ [BEq α] [Hashable α] [EquivBEq α][LawfulHashable α] {m : Raw₀ α β} {l: List ((a : α) × β a)} (h : Raw.WFImp m.1): Raw.WFImp (insertManyListₘ m l).1 := by
+/-! # `insertListₘ` -/
+theorem wfImp_insertListₘ [BEq α] [Hashable α] [EquivBEq α][LawfulHashable α] {m : Raw₀ α β} {l: List ((a : α) × β a)} (h : Raw.WFImp m.1): Raw.WFImp (insertListₘ m l).1 := by
   induction l generalizing m with
   | nil =>
-    simp[insertManyListₘ]
+    simp[insertListₘ]
     exact h
   | cons hd tl ih =>
-    simp[insertManyListₘ]
+    simp[insertListₘ]
     apply ih
     apply wfImp_insert h
 
-theorem toListModel_insertManyListₘ [BEq α] [Hashable α] [EquivBEq α][LawfulHashable α] {m : Raw₀ α β} {l: List ((a : α) × β a)} (h : Raw.WFImp m.1):
-  Perm (toListModel (insertManyListₘ m l).1.buckets) (List.insertMany (toListModel m.1.buckets) l) := by
+theorem toListModel_insertListₘ [BEq α] [Hashable α] [EquivBEq α][LawfulHashable α] {m : Raw₀ α β} {l: List ((a : α) × β a)} (h : Raw.WFImp m.1):
+  Perm (toListModel (insertListₘ m l).1.buckets) (List.insertMany (toListModel m.1.buckets) l) := by
 induction l generalizing m with
 | nil =>
-  simp[insertManyListₘ, List.insertMany]
+  simp[insertListₘ, List.insertMany]
 | cons hd tl ih =>
-  simp[insertManyListₘ, List.insertMany]
+  simp[insertListₘ, List.insertMany]
   apply Perm.trans
   apply ih (wfImp_insert h)
   apply List.insertMany_perm_of_perm_first
   apply toListModel_insert h
   apply (wfImp_insert h).distinct
 
-/-! # `insertManyList` -/
-theorem wfImp_insertManyList [BEq α] [Hashable α] [EquivBEq α][LawfulHashable α] {m : Raw₀ α β} {l: List ((a : α) × β a)} (h : Raw.WFImp m.1): Raw.WFImp (insertManyList m l).1 := by
-  rw [insertManyList_eq_insertManyListₘ]
-  apply wfImp_insertManyListₘ h
+/-! # `insertList` -/
+theorem wfImp_insertList [BEq α] [Hashable α] [EquivBEq α][LawfulHashable α] {m : Raw₀ α β} {l: List ((a : α) × β a)} (h : Raw.WFImp m.1): Raw.WFImp (insertList m l).1 := by
+  rw [insertList_eq_insertListₘ]
+  apply wfImp_insertListₘ h
 
-theorem toListModel_insertManyList [BEq α] [Hashable α] [EquivBEq α][LawfulHashable α] {m : Raw₀ α β} {l: List ((a : α) × β a)} (h : Raw.WFImp m.1):
-  Perm (toListModel (insertManyList m l).1.buckets) (List.insertMany (toListModel m.1.buckets) l) := by
-  rw [insertManyList_eq_insertManyListₘ]
-  apply toListModel_insertManyListₘ h
+theorem toListModel_insertList [BEq α] [Hashable α] [EquivBEq α][LawfulHashable α] {m : Raw₀ α β} {l: List ((a : α) × β a)} (h : Raw.WFImp m.1):
+  Perm (toListModel (insertList m l).1.buckets) (List.insertMany (toListModel m.1.buckets) l) := by
+  rw [insertList_eq_insertListₘ]
+  apply toListModel_insertListₘ h
 
 end Raw₀
 
